---
title: Math285 Final Review
summary: This is the review note for Math285 Final (Spring 2025) by Jiashen Ren.
date: 2025-05-01
author: Jiashen Ren
type: docs
math: true
tags:
  - Math285
---



## Q2:Frobenius method

### Sample Problem

Consider the differential equation

$$2x^2y'' + 3x(x+1)y' - 6y = 0. \qquad \text{(DE)}$$

a) Verify that $x_0 = 0$ is a regular singular point of (DE).

b) Determine the general solution of (DE) on $(0, \infty)$.

c) Using the result of b), state the general solution of (DE) on $(-\infty, 0)$ and on $\mathbb{R}$.

### Background Knowledge

1. **singular point and regular singular point** 

    * $$P(x)y'' + Q(x)y' + R(x)y = 0$$

      if $P(x_0) = 0$, $x_0$ is a singular point

    * $$y'' + p(x)y' + q(x)y = 0$$  
  
      $p(x) = \frac{Q(x)}{P(x)}$,  $q(x) = \frac{R(x)}{P(x)}$
      If $x_0$ is a singular point, and $(x-x_0)p(x)$ and $(x-x_0)^2q(x)$ are finite as $x \to x_0$, then $x_0$ is a regular singular point.

2. Frobenius method

    $$F(r) = r^2 + (P_0 - 1)r + q_0$$

    $P_0 = \lim_{x \to x_0} xp(x)$ and $q_0 = \lim_{x \to x_0} x^2q(x)$

    Solve for $r_1, r_2$

    $$y(x) = (x-x_0)^{r} \sum_{n=0}^{\infty} a_n (x-x_0)^n$$

    Substitute $y(x)$, $y'(x)$, $y''(x)$ into the ODE to solve for $a_n$

    You should obtain a relationship between $a_n$ and $a_{n+1}$ 
    Then solve the sequence

### Solution

a) 
The explicit form of (DE) is

$$y'' + \frac{3(x+1)}{2x}y' - \frac{3}{x^2}y = 0$$

$p(x) := \frac{3}{2} \frac{1}{x} + \frac{3}{2}$ has a pole of order 1 at 0, and $q(x) := -\frac{3}{x^2}$ has a pole of order 2 at 0.  This shows that 0 is a regular singular point of (DE).

b)
**1. Verification of Regular Singular Point and Calculation of Indicial Equation:**

*   **Explicit Form:** First, rewrite the original differential equation (DE) into the standard form:
    $$y'' + p(x)y' + q(x)y = 0$$

    to obtain $p(x)$ and $q(x)$.

*   **Order of Poles:** By observation, $p(x)$ has a pole of order 1 at $x=0$, and $q(x)$ has a pole of order 2 at $x=0$. This confirms that $x=0$ is a regular singular point.
*   **Indicial Equation:** Calculate $p_0$ and $q_0$:

    $$p_0 = \lim_{x \to 0} \left[ x \cdot p(x) \right] = \frac{3}{2}$$

    $$q_0 = \lim_{x \to 0} \left[ x^2 \cdot q(x) \right] = -3$$
    Then, construct the indicial equation:

    $$r^2 + (p_0 - 1)r + q_0 = 0$$

    $$r^2 + (1/2)r - 3 = 0$$

    Solve this quadratic equation to get the roots: $r_1 = 3/2$ and $r_2 = -2$.

**2. Constructing Series Solutions:**

*   **Two Linearly Independent Solutions:** Since the difference between the roots $r_1 - r_ 2 = 3/2 - (-2) = 7/2$ is not an integer, the Frobenius method guarantees two linearly independent series solutions, in the form:

    $$y_1(x) = x^{3/2} \sum_{n=0}^{\infty} a_n x^n = \sum_{n=0}^{\infty} a_n x^{n+3/2}$$ 

    $$y_2(x) = x^{-2} \sum_{n=0}^{\infty} b_n x^n = \sum_{n=0}^{\infty} b_n x^{n-2}$$

    where \(a_0 = b_0 = 1\) (normalization condition).

```markdown
{{</* spoiler text="ğŸ‘‰ Why we need to check the difference between the roots" */>}}

è¿™æ˜¯ Frobenius æ–¹æ³•çš„ä¸€ä¸ªæ ¸å¿ƒç»“è®ºã€‚ è®©æˆ‘è§£é‡Šä¸€ä¸‹ä¸ºä»€ä¹ˆå½“æŒ‡æ ‡æ ¹ä¹‹å·®ä¸æ˜¯æ•´æ•°æ—¶ï¼Œå¯ä»¥ä¿è¯æœ‰ä¸¤ä¸ªçº¿æ€§æ— å…³çš„çº§æ•°è§£ï¼š

**Frobenius æ–¹æ³•çš„åŸºæœ¬æ€æƒ³**

Frobenius æ–¹æ³•å‡è®¾è§£çš„å½¢å¼ä¸ºï¼š

$$
y(x) = (x - x_0)^r \sum_{n=0}^{\infty} a_n (x - x_0)^n = \sum_{n=0}^{\infty} a_n (x - x_0)^{n+r}
$$

å…¶ä¸­ \(x_0\) æ˜¯æ­£åˆ™å¥‡ç‚¹ï¼Œ\(r\) æ˜¯å¾…å®šçš„æŒ‡æ ‡ï¼Œ\(a_n\) æ˜¯ç³»æ•°ã€‚ æˆ‘ä»¬å°†è¿™ä¸ªçº§æ•°ä»£å…¥å¾®åˆ†æ–¹ç¨‹ï¼Œå¹¶é€šè¿‡æ¯”è¾ƒç³»æ•°å¾—åˆ°å…³äº \(r\) çš„æŒ‡æ ‡æ–¹ç¨‹ï¼ˆä¸€ä¸ªäºŒæ¬¡æ–¹ç¨‹ï¼‰å’Œå…³äºç³»æ•° \(a_n\) çš„é€’æ¨å…³ç³»ã€‚

**æŒ‡æ ‡æ–¹ç¨‹å’Œè§£çš„ç»“æ„**

æŒ‡æ ‡æ–¹ç¨‹é€šå¸¸æ˜¯ \(r\) çš„äºŒæ¬¡æ–¹ç¨‹ï¼Œæœ‰ä¸¤ä¸ªæ ¹ \(r_1\) å’Œ \(r_2\) (å‡è®¾ \(r_1 \geq r_2\))ã€‚ è¿™ä¸¤ä¸ªæ ¹å†³å®šäº†è§£çš„ *åŸºæœ¬å½¢å¼*ã€‚

**å…³é”®ï¼šæ ¹çš„å·®çš„å½±å“**

*   **æƒ…å†µ 1ï¼š\(r_1 - r_2\) ä¸æ˜¯æ•´æ•°**

    åœ¨è¿™ç§æƒ…å†µä¸‹ï¼Œæˆ‘ä»¬å¯ä»¥ç›´æ¥å¾—åˆ°ä¸¤ä¸ªçº¿æ€§æ— å…³çš„è§£ï¼š

    *   \(y_1(x) = (x - x_0)^{r_1} \sum_{n=0}^{\infty} a_n (x - x_0)^n\)  (ä½¿ç”¨ \(r_1\) å’Œé€’æ¨å…³ç³»)
    *   \(y_2(x) = (x - x_0)^{r_2} \sum_{n=0}^{\infty} b_n (x - x_0)^n\)  (ä½¿ç”¨ \(r_2\) å’Œé€’æ¨å…³ç³»)

    è¿™ä¸¤ä¸ªè§£åœ¨ \(x=x_0\) é™„è¿‘çš„ leading term ï¼ˆä¸»å¯¼é¡¹ï¼‰åˆ†åˆ«æ˜¯ \((x-x_0)^{r_1}\) å’Œ \((x-x_0)^{r_2}\)ã€‚ å› ä¸º \(r_1\) å’Œ \(r_2\) ä¸åŒï¼Œä¸”å®ƒä»¬çš„å·®ä¸æ˜¯æ•´æ•°ï¼Œè¿™æ„å‘³ç€è¿™ä¸¤ä¸ªçº§æ•° *ä¸å¯èƒ½* é€šè¿‡ä¹˜ä»¥ä¸€ä¸ªå¸¸æ•°è€Œäº’ç›¸è½¬åŒ–ã€‚ ä¹Ÿå°±æ˜¯è¯´ï¼Œå®ƒä»¬æ˜¯çº¿æ€§æ— å…³çš„ã€‚ å…³é”®ç‚¹æ˜¯è¿™ä¸ªéæ•´æ•°å·®ç¡®ä¿çº§æ•°ä¸­çš„æ¯ä¸€é¡¹éƒ½ä¸ä¼šâ€œæŠµæ¶ˆâ€æˆ–â€œé‡å¤â€ã€‚

*   **æƒ…å†µ 2ï¼š\(r_1 = r_2\) (é‡æ ¹)**

    åªæœ‰ä¸€ä¸ªæŒ‡æ ‡æ ¹ã€‚ç›´æ¥ç”¨ Frobenius æ–¹æ³•åªèƒ½æ‰¾åˆ°ä¸€ä¸ªè§£ \(y_1(x)\)ã€‚ç¬¬äºŒä¸ªçº¿æ€§æ— å…³çš„è§£éœ€è¦åŒ…å«å¯¹æ•°é¡¹ï¼ˆlogarithmic termï¼‰ï¼š

    $$
    y_2(x) = y_1(x) \ln(x - x_0) + (x - x_0)^{r_1} \sum_{n=0}^{\infty} b_n (x - x_0)^n
    $$
    æ±‚ç³»æ•°å’Œ \(y_1(x)\) çš„é€’æ¨å…³ç³»æ˜¯ä¸åŒçš„.

*   **æƒ…å†µ 3ï¼š\(r_1 - r_2\) æ˜¯æ­£æ•´æ•°**

    è¿™æ˜¯æœ€å¤æ‚çš„æƒ…å†µã€‚ æˆ‘ä»¬å°è¯•ç”¨è¾ƒå°çš„æ ¹ \(r_2\) æ„é€ è§£ \(y_2(x)\) æ—¶ï¼Œå¯èƒ½ä¼šé‡åˆ°é€’æ¨å…³ç³»â€œå¡ä½â€çš„æƒ…å†µï¼ˆåˆ†æ¯ä¸ºé›¶ï¼‰ã€‚ è¿™æ—¶ï¼Œç¬¬äºŒä¸ªè§£ \(y_2(x)\) å¯èƒ½å…·æœ‰ä»¥ä¸‹ä¸¤ç§å½¢å¼ä¹‹ä¸€ï¼š

    *   **å½¢å¼ 1 (æ— å¯¹æ•°é¡¹):**  \(y_2(x) = (x - x_0)^{r_2} \sum_{n=0}^{\infty} b_n (x - x_0)^n\) (è™½ç„¶è¿™ç§æƒ…å†µè¾ƒå°‘è§ï¼Œä½†ç¡®å®å¯èƒ½å‘ç”Ÿï¼Œæ­¤æ—¶é€’æ¨å…³ç³»â€œå¹¸è¿åœ°â€æ²¡æœ‰å¡ä½)

    *   **å½¢å¼ 2 (æœ‰å¯¹æ•°é¡¹):**
        $$
        y_2(x) = A y_1(x) \ln(x - x_0) + (x - x_0)^{r_2} \sum_{n=0}^{\infty} b_n (x - x_0)^n
        $$
        å…¶ä¸­ \(A\) æ˜¯ä¸€ä¸ªéé›¶å¸¸æ•°ã€‚è¿™ç§æƒ…å†µæ›´å¸¸è§ã€‚

**ç›´è§‚ç†è§£ï¼ˆä¸ºä»€ä¹ˆéæ•´æ•°å·®å¾ˆé‡è¦ï¼‰**

æƒ³è±¡ä¸€ä¸‹ä¸¤ä¸ªçº§æ•°ï¼š

*   \(y_1(x) = x^{3/2} (1 + a_1 x + a_2 x^2 + \ldots)\)
*   \(y_2(x) = x^{-2} (1 + b_1 x + b_2 x^2 + \ldots)\)

\(y_1(x)\) ä¸­çš„å„é¡¹çš„æŒ‡æ•°æ˜¯ \(3/2, 5/2, 7/2, \ldots\)ï¼Œè€Œ \(y_2(x)\) ä¸­çš„å„é¡¹çš„æŒ‡æ•°æ˜¯ \(-2, -1, 0, 1, 2, \ldots\)ã€‚ å› ä¸ºæŒ‡æ•°çš„ *å·®å¼‚* æ°¸è¿œä¸ä¼šæ˜¯æ•´æ•°ï¼Œæ‰€ä»¥ä½ ä¸å¯èƒ½é€šè¿‡è°ƒæ•´ \(y_1(x)\) çš„ç³»æ•°æ¥å¾—åˆ° \(y_2(x)\) ä¸­çš„ä»»ä½•ä¸€é¡¹ã€‚ è¿™å°±æ˜¯çº¿æ€§æ— å…³çš„æœ¬è´¨ã€‚

å¦‚æœå·®æ˜¯æ•´æ•°ï¼Œæ¯”å¦‚ï¼š

*    \(y_1(x) = x^2 (1 + a_1 x + \ldots)\)
*    \(y_2(x) = x^0 (1 + b_1 x + \ldots)\)

é‚£ä¹ˆç†è®ºä¸Šï¼Œ\(y_1\) çš„çº§æ•°éƒ¨åˆ†å’Œ \(y_2\) çš„çº§æ•°éƒ¨åˆ†æœ‰å¯èƒ½é€šè¿‡ä¸åŒçš„ç³»æ•°ç›¸ç­‰ã€‚ è¿™æ—¶å¿…é¡»æ£€æŸ¥é€’æ¨å…¬å¼ã€‚å¦‚æœé€’æ¨å…¬å¼æ— è§£ï¼ˆåˆ†æ¯ä¸º 0ï¼‰ï¼Œå¿…é¡»å¼•å…¥å¯¹æ•°ã€‚

**æ€»ç»“**

å½“æŒ‡æ ‡æ ¹ä¹‹å·®ä¸æ˜¯æ•´æ•°æ—¶ï¼ŒFrobenius æ–¹æ³•ç›´æ¥ç»™å‡ºçš„ä¸¤ä¸ªçº§æ•°è§£ï¼Œç”±äºå…¶é¦–é¡¹ï¼ˆleading termï¼‰çš„æŒ‡æ•°ä¸åŒä¸”å·®ä¸æ˜¯æ•´æ•°ï¼Œä¿è¯äº†å®ƒä»¬æ˜¯çº¿æ€§æ— å…³çš„ã€‚ è¿™æ˜¯ Frobenius æ–¹æ³•çš„ä¸€ä¸ªæ¼‚äº®ä¸”é‡è¦çš„ç»“æœï¼Œä½¿å¾—åœ¨æ­£åˆ™å¥‡ç‚¹é™„è¿‘å¯»æ‰¾çº§æ•°è§£æˆä¸ºå¯èƒ½ã€‚
{{</* /spoiler */>}}
```
**3. Solving for the First Solution y1(x):**

*   **Substitute into Original Equation:** Substitute the series forms of \(y_1(x)\), \(y_1'(x)\), and \(y_1''(x)\) into the original differential equation.
*   **Combine Series:** Combine coefficients of like powers of \(x\).
*   **Recurrence Relation:** By setting the coefficients of each power of \(x\) to zero, obtain the recurrence relation for the coefficients \(a_n\):
    $$
    a_n = -\frac{3(2n + 1)}{2n(2n + 7)} a_{n-1}
    $$
*   **Calculate Coefficients:** Starting from \(a_0 = 1\), use the recurrence relation to calculate \(a_1, a_2, a_3, \ldots\).
*   **Write \(y_1(x)\):** Substitute the calculated coefficients into the series expression for \(y_1(x)\).

**4. Solving for the Second Solution \(y_2(x)\):**

*   **Repeat Steps:** Repeat the above process for \(y_2(x)\) (substitution, combination, recurrence).
*   **Recurrence Relation:** Obtain the recurrence relation for \(b_n\):
    $$
    b_n = \frac{3(n - 3)}{n(2n - 7)} b_{n-1}
    $$
*   **Calculate Coefficients:** Starting from \(b_0 = 1\), use the recurrence relation to calculate \(b_1, b_2, b_3, \ldots\). Note that \(b_3, b_4, \ldots\) are zero.
*   **Write \(y_2(x)\):** Substitute the calculated coefficients into the series expression for \(y_2(x)\).

**5. General Solution:**

Finally, the general solution of the differential equation is the linear combination of \(y_1(x)\) and \(y_2(x)\):

$$
y(x) = C_1 y_1(x) + C_2 y_2(x)
$$

where \(C_1\) and \(C_2\) are arbitrary constants.

---
**Alternative solution:**

---
