---
title: âœ… Math285 Final Review
summary: This is the review note for Math285 Final (Spring 2025) by Jiashen Ren.
date: 2025-02-07
authors:
  - admin
tags:
  - Math285
image:
  caption: 'Math285 Class'
---

## Q2:Frobenius method

### Sample Problem

Consider the differential equation

$$2x^2y'' + 3x(x+1)y' - 6y = 0. \qquad \text{(DE)}$$

a) Verify that $x_0 = 0$ is a regular singular point of (DE).

b) Determine the general solution of (DE) on $(0, \infty)$.

c) Using the result of b), state the general solution of (DE) on $(-\infty, 0)$ and on $\mathbb{R}$.

### Background Knowledge

1. **singular point and regular singular point** 

    * $$P(x)y'' + Q(x)y' + R(x)y = 0$$

      if $P(x_0) = 0$, $x_0$ is a singular point

    * $$y'' + p(x)y' + q(x)y = 0$$  
  
      $p(x) = \frac{Q(x)}{P(x)}$,  $q(x) = \frac{R(x)}{P(x)}$
      If $x_0$ is a singular point, and $(x-x_0)p(x)$ and $(x-x_0)^2q(x)$ are finite as $x \to x_0$, then $x_0$ is a regular singular point.

2. Frobenius method

    $$F(r) = r^2 + (P_0 - 1)r + q_0$$

    $P_0 = \lim_{x \to x_0} xp(x)$ and $q_0 = \lim_{x \to x_0} x^2q(x)$

    Solve for $r_1, r_2$

    $$y(x) = (x-x_0)^{r} \sum_{n=0}^{\infty} a_n (x-x_0)^n$$

    Substitute $y(x)$, $y'(x)$, $y''(x)$ into the ODE to solve for $a_n$

    You should obtain a relationship between $a_n$ and $a_{n+1}$ 
    Then solve the sequence

### Solution

a) 
The explicit form of (DE) is

$$y'' + \frac{3(x+1)}{2x}y' - \frac{3}{x^2}y = 0$$

$p(x) := \frac{3}{2} \frac{1}{x} + \frac{3}{2}$ has a pole of order 1 at 0, and $q(x) := -\frac{3}{x^2}$ has a pole of order 2 at 0.  This shows that 0 is a regular singular point of (DE).

b)
**1. Verification of Regular Singular Point and Calculation of Indicial Equation:**

*   **Explicit Form:** First, rewrite the original differential equation (DE) into the standard form:
    $$y'' + p(x)y' + q(x)y = 0$$

    to obtain $p(x)$ and $q(x)$.

*   **Order of Poles:** By observation, $p(x)$ has a pole of order 1 at $x=0$, and $q(x)$ has a pole of order 2 at $x=0$. This confirms that $x=0$ is a regular singular point.
*   **Indicial Equation:** Calculate $p_0$ and $q_0$:

    $$p_0 = \lim_{x \to 0} \left[ x \cdot p(x) \right] = \frac{3}{2}$$

    $$q_0 = \lim_{x \to 0} \left[ x^2 \cdot q(x) \right] = -3$$
    Then, construct the indicial equation:

    $$r^2 + (p_0 - 1)r + q_0 = 0$$

    $$r^2 + (1/2)r - 3 = 0$$

    Solve this quadratic equation to get the roots: $r_1 = 3/2$ and $r_2 = -2$.

**2. Constructing Series Solutions:**

*   **Two Linearly Independent Solutions:** Since the difference between the roots $r_1 - r_ 2 = 3/2 - (-2) = 7/2$ is not an integer, the Frobenius method guarantees two linearly independent series solutions, in the form:

    $$y_1(x) = x^{3/2} \sum_{n=0}^{\infty} a_n x^n = \sum_{n=0}^{\infty} a_n x^{n+3/2}$$ 

    $$y_2(x) = x^{-2} \sum_{n=0}^{\infty} b_n x^n = \sum_{n=0}^{\infty} b_n x^{n-2}$$

    where \(a_0 = b_0 = 1\) (normalization condition).


{{< spoiler text="ğŸ‘‰ Why we need to check the difference between the roots" >}}

è¿™æ˜¯ Frobenius æ–¹æ³•çš„ä¸€ä¸ªæ ¸å¿ƒç»“è®ºã€‚ è®©æˆ‘è§£é‡Šä¸€ä¸‹ä¸ºä»€ä¹ˆå½“æŒ‡æ ‡æ ¹ä¹‹å·®ä¸æ˜¯æ•´æ•°æ—¶ï¼Œå¯ä»¥ä¿è¯æœ‰ä¸¤ä¸ªçº¿æ€§æ— å…³çš„çº§æ•°è§£ï¼š

**Frobenius æ–¹æ³•çš„åŸºæœ¬æ€æƒ³**

Frobenius æ–¹æ³•å‡è®¾è§£çš„å½¢å¼ä¸ºï¼š

$$
y(x) = (x - x_0)^r \sum_{n=0}^{\infty} a_n (x - x_0)^n = \sum_{n=0}^{\infty} a_n (x - x_0)^{n+r}
$$

å…¶ä¸­ \(x_0\) æ˜¯æ­£åˆ™å¥‡ç‚¹ï¼Œ\(r\) æ˜¯å¾…å®šçš„æŒ‡æ ‡ï¼Œ\(a_n\) æ˜¯ç³»æ•°ã€‚ æˆ‘ä»¬å°†è¿™ä¸ªçº§æ•°ä»£å…¥å¾®åˆ†æ–¹ç¨‹ï¼Œå¹¶é€šè¿‡æ¯”è¾ƒç³»æ•°å¾—åˆ°å…³äº \(r\) çš„æŒ‡æ ‡æ–¹ç¨‹ï¼ˆä¸€ä¸ªäºŒæ¬¡æ–¹ç¨‹ï¼‰å’Œå…³äºç³»æ•° \(a_n\) çš„é€’æ¨å…³ç³»ã€‚

**æŒ‡æ ‡æ–¹ç¨‹å’Œè§£çš„ç»“æ„**

æŒ‡æ ‡æ–¹ç¨‹é€šå¸¸æ˜¯ \(r\) çš„äºŒæ¬¡æ–¹ç¨‹ï¼Œæœ‰ä¸¤ä¸ªæ ¹ \(r_1\) å’Œ \(r_2\) (å‡è®¾ \(r_1 \geq r_2\))ã€‚ è¿™ä¸¤ä¸ªæ ¹å†³å®šäº†è§£çš„ *åŸºæœ¬å½¢å¼*ã€‚

**å…³é”®ï¼šæ ¹çš„å·®çš„å½±å“**

*   **æƒ…å†µ 1ï¼š\(r_1 - r_2\) ä¸æ˜¯æ•´æ•°**

    åœ¨è¿™ç§æƒ…å†µä¸‹ï¼Œæˆ‘ä»¬å¯ä»¥ç›´æ¥å¾—åˆ°ä¸¤ä¸ªçº¿æ€§æ— å…³çš„è§£ï¼š

    *   \(y_1(x) = (x - x_0)^{r_1} \sum_{n=0}^{\infty} a_n (x - x_0)^n\)  (ä½¿ç”¨ \(r_1\) å’Œé€’æ¨å…³ç³»)
    *   \(y_2(x) = (x - x_0)^{r_2} \sum_{n=0}^{\infty} b_n (x - x_0)^n\)  (ä½¿ç”¨ \(r_2\) å’Œé€’æ¨å…³ç³»)

    è¿™ä¸¤ä¸ªè§£åœ¨ \(x=x_0\) é™„è¿‘çš„ leading term ï¼ˆä¸»å¯¼é¡¹ï¼‰åˆ†åˆ«æ˜¯ \((x-x_0)^{r_1}\) å’Œ \((x-x_0)^{r_2}\)ã€‚ å› ä¸º \(r_1\) å’Œ \(r_2\) ä¸åŒï¼Œä¸”å®ƒä»¬çš„å·®ä¸æ˜¯æ•´æ•°ï¼Œè¿™æ„å‘³ç€è¿™ä¸¤ä¸ªçº§æ•° *ä¸å¯èƒ½* é€šè¿‡ä¹˜ä»¥ä¸€ä¸ªå¸¸æ•°è€Œäº’ç›¸è½¬åŒ–ã€‚ ä¹Ÿå°±æ˜¯è¯´ï¼Œå®ƒä»¬æ˜¯çº¿æ€§æ— å…³çš„ã€‚ å…³é”®ç‚¹æ˜¯è¿™ä¸ªéæ•´æ•°å·®ç¡®ä¿çº§æ•°ä¸­çš„æ¯ä¸€é¡¹éƒ½ä¸ä¼šâ€œæŠµæ¶ˆâ€æˆ–â€œé‡å¤â€ã€‚

*   **æƒ…å†µ 2ï¼š\(r_1 = r_2\) (é‡æ ¹)**

    åªæœ‰ä¸€ä¸ªæŒ‡æ ‡æ ¹ã€‚ç›´æ¥ç”¨ Frobenius æ–¹æ³•åªèƒ½æ‰¾åˆ°ä¸€ä¸ªè§£ \(y_1(x)\)ã€‚ç¬¬äºŒä¸ªçº¿æ€§æ— å…³çš„è§£éœ€è¦åŒ…å«å¯¹æ•°é¡¹ï¼ˆlogarithmic termï¼‰ï¼š

    $$
    y_2(x) = y_1(x) \ln(x - x_0) + (x - x_0)^{r_1} \sum_{n=0}^{\infty} b_n (x - x_0)^n
    $$
    æ±‚ç³»æ•°å’Œ \(y_1(x)\) çš„é€’æ¨å…³ç³»æ˜¯ä¸åŒçš„.

*   **æƒ…å†µ 3ï¼š\(r_1 - r_2\) æ˜¯æ­£æ•´æ•°**

    è¿™æ˜¯æœ€å¤æ‚çš„æƒ…å†µã€‚ æˆ‘ä»¬å°è¯•ç”¨è¾ƒå°çš„æ ¹ \(r_2\) æ„é€ è§£ \(y_2(x)\) æ—¶ï¼Œå¯èƒ½ä¼šé‡åˆ°é€’æ¨å…³ç³»â€œå¡ä½â€çš„æƒ…å†µï¼ˆåˆ†æ¯ä¸ºé›¶ï¼‰ã€‚ è¿™æ—¶ï¼Œç¬¬äºŒä¸ªè§£ \(y_2(x)\) å¯èƒ½å…·æœ‰ä»¥ä¸‹ä¸¤ç§å½¢å¼ä¹‹ä¸€ï¼š

    *   **å½¢å¼ 1 (æ— å¯¹æ•°é¡¹):**  \(y_2(x) = (x - x_0)^{r_2} \sum_{n=0}^{\infty} b_n (x - x_0)^n\) (è™½ç„¶è¿™ç§æƒ…å†µè¾ƒå°‘è§ï¼Œä½†ç¡®å®å¯èƒ½å‘ç”Ÿï¼Œæ­¤æ—¶é€’æ¨å…³ç³»â€œå¹¸è¿åœ°â€æ²¡æœ‰å¡ä½)

    *   **å½¢å¼ 2 (æœ‰å¯¹æ•°é¡¹):**
        $$
        y_2(x) = A y_1(x) \ln(x - x_0) + (x - x_0)^{r_2} \sum_{n=0}^{\infty} b_n (x - x_0)^n
        $$
        å…¶ä¸­ \(A\) æ˜¯ä¸€ä¸ªéé›¶å¸¸æ•°ã€‚è¿™ç§æƒ…å†µæ›´å¸¸è§ã€‚

**ç›´è§‚ç†è§£ï¼ˆä¸ºä»€ä¹ˆéæ•´æ•°å·®å¾ˆé‡è¦ï¼‰**

æƒ³è±¡ä¸€ä¸‹ä¸¤ä¸ªçº§æ•°ï¼š

*   \(y_1(x) = x^{3/2} (1 + a_1 x + a_2 x^2 + \ldots)\)
*   \(y_2(x) = x^{-2} (1 + b_1 x + b_2 x^2 + \ldots)\)

\(y_1(x)\) ä¸­çš„å„é¡¹çš„æŒ‡æ•°æ˜¯ \(3/2, 5/2, 7/2, \ldots\)ï¼Œè€Œ \(y_2(x)\) ä¸­çš„å„é¡¹çš„æŒ‡æ•°æ˜¯ \(-2, -1, 0, 1, 2, \ldots\)ã€‚ å› ä¸ºæŒ‡æ•°çš„ *å·®å¼‚* æ°¸è¿œä¸ä¼šæ˜¯æ•´æ•°ï¼Œæ‰€ä»¥ä½ ä¸å¯èƒ½é€šè¿‡è°ƒæ•´ \(y_1(x)\) çš„ç³»æ•°æ¥å¾—åˆ° \(y_2(x)\) ä¸­çš„ä»»ä½•ä¸€é¡¹ã€‚ è¿™å°±æ˜¯çº¿æ€§æ— å…³çš„æœ¬è´¨ã€‚

å¦‚æœå·®æ˜¯æ•´æ•°ï¼Œæ¯”å¦‚ï¼š

*    \(y_1(x) = x^2 (1 + a_1 x + \ldots)\)
*    \(y_2(x) = x^0 (1 + b_1 x + \ldots)\)

é‚£ä¹ˆç†è®ºä¸Šï¼Œ\(y_1\) çš„çº§æ•°éƒ¨åˆ†å’Œ \(y_2\) çš„çº§æ•°éƒ¨åˆ†æœ‰å¯èƒ½é€šè¿‡ä¸åŒçš„ç³»æ•°ç›¸ç­‰ã€‚ è¿™æ—¶å¿…é¡»æ£€æŸ¥é€’æ¨å…¬å¼ã€‚å¦‚æœé€’æ¨å…¬å¼æ— è§£ï¼ˆåˆ†æ¯ä¸º 0ï¼‰ï¼Œå¿…é¡»å¼•å…¥å¯¹æ•°ã€‚

**æ€»ç»“**

å½“æŒ‡æ ‡æ ¹ä¹‹å·®ä¸æ˜¯æ•´æ•°æ—¶ï¼ŒFrobenius æ–¹æ³•ç›´æ¥ç»™å‡ºçš„ä¸¤ä¸ªçº§æ•°è§£ï¼Œç”±äºå…¶é¦–é¡¹ï¼ˆleading termï¼‰çš„æŒ‡æ•°ä¸åŒä¸”å·®ä¸æ˜¯æ•´æ•°ï¼Œä¿è¯äº†å®ƒä»¬æ˜¯çº¿æ€§æ— å…³çš„ã€‚ è¿™æ˜¯ Frobenius æ–¹æ³•çš„ä¸€ä¸ªæ¼‚äº®ä¸”é‡è¦çš„ç»“æœï¼Œä½¿å¾—åœ¨æ­£åˆ™å¥‡ç‚¹é™„è¿‘å¯»æ‰¾çº§æ•°è§£æˆä¸ºå¯èƒ½ã€‚
{{< /spoiler >}}

**3. Solving for the First Solution y1(x):**

*   **Substitute into Original Equation:** Substitute the series forms of \(y_1(x)\), \(y_1'(x)\), and \(y_1''(x)\) into the original differential equation.
*   **Combine Series:** Combine coefficients of like powers of \(x\).
*   **Recurrence Relation:** By setting the coefficients of each power of \(x\) to zero, obtain the recurrence relation for the coefficients \(a_n\):
    $$
    a_n = -\frac{3(2n + 1)}{2n(2n + 7)} a_{n-1}
    $$
*   **Calculate Coefficients:** Starting from \(a_0 = 1\), use the recurrence relation to calculate \(a_1, a_2, a_3, \ldots\).
*   **Write \(y_1(x)\):** Substitute the calculated coefficients into the series expression for \(y_1(x)\).

**4. Solving for the Second Solution \(y_2(x)\):**

*   **Repeat Steps:** Repeat the above process for \(y_2(x)\) (substitution, combination, recurrence).
*   **Recurrence Relation:** Obtain the recurrence relation for \(b_n\):
    $$
    b_n = \frac{3(n - 3)}{n(2n - 7)} b_{n-1}
    $$
*   **Calculate Coefficients:** Starting from \(b_0 = 1\), use the recurrence relation to calculate \(b_1, b_2, b_3, \ldots\). Note that \(b_3, b_4, \ldots\) are zero.
*   **Write \(y_2(x)\):** Substitute the calculated coefficients into the series expression for \(y_2(x)\).

**5. General Solution:**

Finally, the general solution of the differential equation is the linear combination of \(y_1(x)\) and \(y_2(x)\):

$$
y(x) = C_1 y_1(x) + C_2 y_2(x)
$$

where \(C_1\) and \(C_2\) are arbitrary constants.

---
**Alternative solution:**

\[
a_n(r) \;=\; -\,\frac{1}{F\bigl(r+n\bigr)} \;\sum_{k=0}^{n-1} \Bigl[\bigl(r+k\bigr)\,p_{n-k} \;+\; q_{n-k}\Bigr]\,a_k(r),
\quad
a_0(r) \;=\; 1,
\]
where
\[
F(r) \;=\; \bigl(r - \tfrac{3}{2}\bigr)\,\bigl(r + 2\bigr),
\]
and all \(p_i,\,q_i=0\) except \(p_0 = p_1 = \tfrac{3}{2}\) and \(q_0 = -3.\)

â€¢ **Stepâ€¯1: Substitute \(F(r+n)\).**  
Replace \(F(r+n)\) with \(\bigl(r + n - \tfrac{3}{2}\bigr)\,\bigl(r + n + 2\bigr).\)

â€¢ **Stepâ€¯2: Handle the Summation.**  
For \(n=1\):
\[
a_1(r)
=\;
-\,\frac{1}{\bigl(r+1 - \tfrac{3}{2}\bigr)\,\bigl(r+1+2\bigr)}
\;\bigl[\,(r)\,p_1 + q_1\bigr]\,a_0(r).
\]
Given \(p_1=\tfrac{3}{2}\) and \(q_1=0\), we get
\[
a_1(r)
=\;
-\,\frac{\tfrac{3}{2}\,r}{\bigl(r - \tfrac{1}{2}\bigr)\,\bigl(r+3\bigr)}.
\]

For \(n\ge2\), the only nonzero terms in the sum occur when \(n-k=1\). Hence,
\[
a_n(r)
=\;
-\,\frac{(r + n - 1)\,\tfrac{3}{2}}{\bigl(r+n - \tfrac{3}{2}\bigr)\,\bigl(r+n+2\bigr)}
\,a_{n-1}(r).
\]

â€¢ **Stepâ€¯3: Iterate (and find a pattern).**  
By applying the recurrence repeatedly, we see a pattern emerge for \(a_n(r)\).  

â€¢ **Stepâ€¯4: Generalize.**  
A typical closed form (for \(n\ge4\)) looks like
\[
a_n(r)
=\;
(-1)^n\,3^n
\,\frac{r\,(r+1)\cdots(r+n-1)}{\bigl(2r-1\bigr)\,\bigl(2r+1\bigr)\cdots\bigl(2r+2n-3\bigr)\,\bigl(r+3\bigr)\,\bigl(r+4\bigr)\cdots\bigl(r+n+2\bigr)}.
\]

### Summary

1. **Two Independent Solutions**  
    Substitute \(r_1=\tfrac{3}{2}\) and \(r_2=-2\) into the recurrence to get two sets of coefficients \(\{a_n(r_1)\}\) and \(\{a_n(r_2)\}\). These form two linearly independent series solutions, \(y_1(x)\) and \(y_2(x)\).

2. **General Solution**  
    Since this is a second-order linear ODE, the full solution on \((0,\infty)\) is
    \[
    y(x) \;=\; c_1\,y_1(x) \;+\; c_2\,y_2(x),
    \]
    where \(c_1\) and \(c_2\) are constants.

3. **Interval of Validity**  
    The coefficients \(p(x)\) and \(q(x)\) are analytic on \(\mathbb{C}\setminus\{0\}\). Because the radius of convergence is infinite and the only singularity is at \(x=0\), the series solution is valid for \(x>0\), i.e. \((0,\infty)\).

---

c) 

**Methodology Summary**

1. **Identify Equation Type and Singularities:**  
First, identify the type of the given differential equation (e.g., second-order linear with constant/variable coefficients). The key is to identify the **singular points** of the equation, especially **regular singular points**. Problem (a) explicitly states that $x = 0$ is a regular singular point.

2. **Solve Near the Singular Point (Usually Using the Frobenius Method):**  
For regular singular points, we typically use the **Frobenius method** (or generalized power series method) to find series solutions near the singular point. This usually involves:  
â€¢ Assuming a solution of the form $y(x) = x^r \sum_{n=0}^{\infty} a_n x^n$.  
â€¢ Substituting the assumed solution into the differential equation.  
â€¢ By comparing coefficients of like powers of $x$, obtaining the **indicial equation** (for $r$) and a recurrence relation for $a_n$.  
â€¢ Solving the indicial equation to get the roots $r_1, r_2$.  
â€¢ Based on the nature of the roots (real and distinct, real and equal, or complex), obtaining the corresponding **fundamental set of solutions** $y_1(x)$ and $y_2(x)$. Note that these solutions are usually solutions near the singular point (e.g., $x > 0$ or $x < 0$). Problem (b) is about solving for the solution on $(0, \infty)$.

3. **Consider the Domain and Extension of Solutions:**  
â€¢ **Local vs. Global Solutions:** The solutions obtained by the Frobenius method are usually local solutions near the singular point. We need to consider how to extend these solutions to a larger domain.  
â€¢ **Piecewise Domains:** For intervals containing the singular point, we might need to consider the solution piecewise. For example, solving separately on $(0, \infty)$ and $(-\infty, 0)$. Problem (c) asks for the solutions on $(-\infty, 0)$ and on $\mathbb{R}$.  
â€¢ **Properties at the Singular Point:** At the singular point (e.g., $x = 0$), the properties of the solution might be special. The solution might not be differentiable everywhere, or even continuously differentiable. We need to analyze the continuity and differentiability of the solution at the singular point to determine if the solution can be extended to a larger interval containing the singular point.

4. **Analyze Uniqueness and Linear Combinations of Solutions:**  
The general solution of a linear homogeneous differential equation is a linear combination of the fundamental set of solutions. On a specific interval, the form of the general solution is determined. We need to pay attention to the **uniqueness** of the solution and how to construct the general solution from the fundamental set.

5. **Pay Special Attention to the Influence of Singularities:**  
Singular points are crucial to the behavior of solutions to differential equations. At singular points, the properties of the solution might be different from those at other points. For example, the solution might exhibit singularities (unboundedness, non-differentiability, etc.). Understanding the influence of singularities on the solution is central to solving these types of problems.

**Problem (c): Using the result of (b), state the general solution of (DE) on $(-\infty, 0)$ and on $\mathbb{R}$.**

1. **General Solution on $(-\infty, 0)$:**  
â€¢ **Given Information:** The problem explicitly states that the solution on $(-\infty, 0)$ is $y(x) = c_1\,y_1^-(x) + c_2\,y_2^-(x)$, and $y_2^-(x)$ is the same function as $y_2(x)$ in (b).  
â€¢ **Understanding $y_1^-(x)$:** $$y_1^-(x) = (-x)^{3/2} \sum_{n=0}^{\infty} a_n x^n = |x|^{3/2} \sum_{n=0}^{\infty} a_n x^n.$$ 

The term $(-x)$ appears in the power function because we are considering the case $x < 0$, to ensure that the value under the square root is positive. $|x|^{3/2}$ is also used to emphasize the case for $x < 0$.  
â€¢ **Summary of the General Solution on $(-\infty, 0)$:**  
Therefore, on $(-\infty, 0)$, the form of the general solution is similar to that on $(0, \infty)$, but the form of the fundamental set is slightly different, mainly in the form of $y_1^-(x)$. A common student mistake is to directly use $y_1(x)$ and $y_2(x)$ obtained in (b) as the solution on $(-\infty, 0)$, which is incorrect. Because $y_1(x)$ is defined for $x > 0$, applying it directly is inappropriate. The problem has clearly given the form of $y_1^-(x)$, and we should use it directly.

So, for $(-\infty, 0)$, the general solution is $y(x) = c_1\,y_1^-(x) + c_2\,y_2(x)$, where $y_1^-(x) = |x|^{3/2} \sum_{n=0}^{\infty} a_n x^n$ (the specific series form needs to be obtained by solving using the Frobenius method; the problem only gives the form here), and $y_2(x)$ is the second fundamental solution obtained in (b).

2. **General Solution on $\mathbb{R}$:**  
â€¢ **Given Information:** The problem explicitly states that many students incorrectly claim that the solution on $\mathbb{R}$ is a piecewise function:

$$
x \mapsto
\begin{cases}
y_1(x), & x > 0,\\
0, & x = 0,\\
y_1^{-}(x), & x < 0
\end{cases}
$$

and points out that this solution is **incorrect**.  
â€¢ **Analysis of the Error:** The key explanation in the problem is: â€œSince $y_1(x) \approx x^{3/2}$ for $x \downarrow 0$, the (unique) continuous extension of $y_1(x)$ to $[0,\infty)$ (obtained by setting $y_1(0) = 0$) is **not** twice differentiable at $x = 0$ (only once differentiable).â€  
  - **Continuity:** For the solution to be meaningful on $\mathbb{R}$, we need to ensure that the solution is continuous at $x = 0$. If $\lim_{x\to 0^+} y_1(x) = 0$ and $\lim_{x\to 0^-} y_1^-(x) = 0$, and we define $y(0) = 0$, then this piecewise function is continuous at $x = 0$. The problem mentions $y_1(0) = 0$ to ensure continuity.  
  - **Differentiability:** The differential equation is second-order, so the solution must be **twice differentiable** on $\mathbb{R}$. The problem points out that $y_1(x)$ (and $y_1^-(x)$) is **not** twice differentiable at $x = 0$, only once differentiable. This is because $y_1(x) \approx x^{3/2}$, and its second derivative will approach infinity (or not exist) near $x = 0$.  
  - **Requirements for Solutions of Differential Equations:** The solution of a differential equation must satisfy the differential equation itself. If a function is not twice differentiable, it cannot be a solution of a second-order differential equation (at the points where the second derivative does not exist).

â€¢ **Correct Conclusion:**  
Since neither $y_1(x)$ nor $y_2(x)$ (and neither $y_1^-(x)$ nor $y_2^-(x)$) can maintain twice differentiability at $x = 0$ (unless it is the trivial solution $y(x) \equiv 0$), therefore, the only possible solution on the entire real line $\mathbb{R}$ is the trivial solution $y(x) \equiv 0$. The last sentence in the problem, â€œhence the only solution on $[0,\infty)$, and hence on $\mathbb{R}$, is $y(x) \equiv 0$,â€ confirms this conclusion.

**Summary of the Answer to (c):**  
â€¢ **General Solution on $(-\infty, 0)$:** $y(x) = c_1\,y_1^-(x) + c_2\,y_2(x)$, where $y_1^-(x) = |x|^{3/2} \sum_{n=0}^{\infty} a_n x^n$, and $y_2(x)$ is the second fundamental solution obtained in (b).  
â€¢ **General Solution on $\mathbb{R}$:** $y(x) \equiv 0$ (the zero solution). This is because non-trivial solutions cannot maintain twice differentiability at $x = 0$, and thus do not satisfy the requirement for solutions of the differential equation on $\mathbb{R}$.

### Q3 